Added inpss_invar to while loop invariant, as this includes uniq, which is needed to know when game isn't done. This in turn allows lemmas about when game is/is not done.
Constructive proof that conversion from total ordering to permutation
is injective.

Defined operator that turns permutation into total ordering, but
haven't proved it works properly yet. This is used for proof
of surjectivity of operator taking total ordering to permutation.

Two lemmas about sorted lists still need to be proved, presumably
by induction.

Pulled steps of proof of main lemma into named lemmas.

work-in-progress/deploy-sorting/SortingLB.ec
@@ -37,6 +37,11 @@ proof.
 rewrite (ltr_le_trans 1) // ge1_len.
 qed.
 
+lemma ge0_len : 0 <= len.
+proof.
+rewrite (ler_trans 1) // ge1_len.
+qed.
+
 (* to represent this problem using our framework, we encode queries
    (i, j), for 0 <= i, j < len, as integers between 0 and arity - 1,
    for arity = len * len: *)
@@ -46,6 +51,11 @@ op arity : int = len * len.
 lemma ge1_arity : 1 <= arity.
 proof.
 rewrite /arity mulr_ege1 ge1_len.
+qed.
+
+lemma ge0_arity : 0 <= arity.
+proof.
+rewrite (ler_trans 1) // ge1_arity.
 qed.
 
 (* enc and dec take us back and forth between pairs (i, j) : int *
@@ -178,24 +188,26 @@ type aux = unit.  (* no auxiliary information *)
 op good (aux : aux, xs : inp list) : bool =
   total_ordering xs.
 
-  (* sort with total ordering*)
+(* sort with total ordering *)
 
-op cmp_of_rel (xs: inp list) (x , y : int) : bool =
-  if (0 <= x < len /\ 0 <= y < len)
-  then rel xs x y
-  else  if (0 <= x < len) then true
-  else  if (0 <= y < len) then false
-  else  x <= y.
+op cmp_of_rel (xs : inp list) (x y : int) : bool =
+  if 0 <= x < len /\ 0 <= y < len
+    then rel xs x y
+  else if 0 <= x < len
+    then true
+  else if 0 <= y < len
+    then false
+  else x <= y.
 
 op nosmt cmp_total_ordering (xs: inp list) : bool =
   size xs = arity /\
   (forall (i : int), cmp_of_rel xs i i) /\
   (forall (i j k : int),
-  cmp_of_rel xs i j => cmp_of_rel xs j k => cmp_of_rel xs i k) /\
+   cmp_of_rel xs i j => cmp_of_rel xs j k => cmp_of_rel xs i k) /\
   (forall (i j : int),
-  cmp_of_rel xs i j => cmp_of_rel xs j i => i = j) /\
-  forall (i j : int),
-  i <> j => cmp_of_rel xs i j \/ cmp_of_rel xs j i.
+   cmp_of_rel xs i j => cmp_of_rel xs j i => i = j) /\
+  (forall (i j : int),
+   i <> j => cmp_of_rel xs i j \/ cmp_of_rel xs j i).
 
 lemma cmp_total_ordering_size (xs : inp list) :
   cmp_total_ordering xs => size xs = arity.
@@ -221,10 +233,9 @@ lemma cmp_total_ordering_total (xs : inp list, i j : int) :
 proof. rewrite /cmp_total_ordering /#. qed.
 
 lemma cmp_total_ordering_ne_not_sym (xs : inp list, i j : int) :
-  cmp_total_ordering xs =>i <> j =>
+  cmp_total_ordering xs => i <> j =>
   cmp_of_rel xs i j => ! cmp_of_rel xs j i.
 proof. rewrite /cmp_total_ordering /#. qed.
-  
 
 lemma tot_cmp_tot (xs:inp list):
   total_ordering xs => cmp_total_ordering (xs).
@@ -233,91 +244,266 @@ rewrite /cmp_total_ordering /total_ordering => //.
 smt().
 qed.    
 
-op tsort (xs: inp list) (s: int list) =
-   sort ( cmp_of_rel xs  ) s.
+(* sort using the comparision function of a total ordering *)
 
-op tsorted (xs: inp list) (s: int list) =
-   sorted ( cmp_of_rel xs ) s.
+op tsort (xs : inp list) (bs : int list) : int list =
+   sort (cmp_of_rel xs) bs.
 
+(* test whether sorted using the comparision function of a total ordering *)
 
-lemma sorted_perm_exists (xs : inp list) :
-  total_ordering xs =>
-  exists (perm : int list),
-  perm_eq (range 0 len) perm /\ tsorted xs perm.
+op tsorted (xs: inp list) (bs : int list) : bool =
+   sorted (cmp_of_rel xs) bs.
+
+(* the list 0 .. len - 1 *)
+
+op range_len : int list = range 0 len.
+
+(* all permutations of 0 .. len - 1 *)
+
+op perms_len : int list list = allperms range_len.
+
+lemma size_perms_len : size perms_len = fact len.
 proof.
-move => tot_ord_xs.
-exists (sort (cmp_of_rel xs) (range 0 len )).
-split.
-smt(perm_eq_sym perm_sort).
-rewrite /tsorted.
-rewrite (sort_sorted).
-smt(tot_cmp_tot cmp_total_ordering_total).
+by rewrite /perms_len size_allperms_uniq /range_len 1:range_uniq
+          size_range /= ler_maxr 1:ge0_len.
 qed.
 
-lemma diff_equal_size_least_index_diff (xs ys : 'a list) :
+(* convert a total ordering into a permutation on 0 .. len - 1 *)
+
+op total_ordering_to_perm_len (xs : inp list) : int list =
+  tsort xs range_len.
+
+lemma sorted_nth (ms : 'a list, e : 'a -> 'a -> bool, k l : int) :
+  (forall (x y : 'a), e x y \/ e y x) =>
+  (forall (y x z : 'a), e x y => e y z => e x z) =>
+  (forall (x y : 'a), e x y => e y x => x = y) =>
+  sorted e ms => 0 <= k <= l < size ms =>
+  e (nth witness ms k) (nth witness ms l).
+proof.
+move => tot_e trans_e antisym_e.
+elim ms.
+rewrite /= /#.
+move => x xs IH /=.
+admit.
+qed.
+
+lemma sorted_exists_nth (ms : 'a list, e : 'a -> 'a -> bool, x y : 'a) :
+  (forall (x y : 'a), e x y \/ e y x) =>
+  (forall (y x z : 'a), e x y => e y z => e x z) =>
+  (forall (x y : 'a), e x y => e y x => x = y) =>
+  sorted e ms => x \in ms => y \in ms => e x y =>
+  exists (k l : int),
+  0 <= k < size ms /\ 0 <= l < size ms /\ k <= l /\
+  nth witness ms k = x /\ nth witness ms l = y.
+proof.
+admit.
+qed.
+
+lemma diff_equal_size_index_diff (xs ys : bool list) :
   xs <> ys => size xs = size ys => 
   (exists (i : int),
-   0 <= i < size xs /\ nth witness xs i <> nth witness ys i /\
-   (forall (j : int),
-    0 <= j < i => nth witness xs j = nth witness ys j)).
+   0 <= i < size xs /\ nth false xs i <> nth false ys i).
 proof.
 move => eq_size ne_xs_ys.
-pose P :=
-  fun (i : int) =>
-  i < size xs /\ nth witness xs i <> nth witness ys i.
-have /# := pmin_spec P _.
-  rewrite /sempty /pcap /P negb_forall /=.
-  case
-    (exists i,
-     0 <= i < size xs /\
-     nth witness xs i <> nth witness ys i) => [/# |].
-  rewrite negb_exists /= => H.
-  have // := eq_from_nth witness xs ys _ _.
-    trivial. smt().
+case
+  (exists i,
+   (0 <= i && i < size xs) /\ nth false xs i <> nth false ys i) =>
+  [// |].
+have -> H :
+  (! (exists (i : int),
+      (0 <= i && i < size xs) /\ nth false xs i <> nth false ys i)) =
+  (forall (i : int), 0 <= i < size xs => nth false xs i = nth false ys i).
+  smt().
+have // : xs = ys.
+by rewrite (eq_from_nth false xs ys).
 qed.
 
-
-op sorted_perm_len_rel (xs : inp list, perm : int list) : bool =
-  perm_eq (range 0 len) perm /\ tsorted xs perm.
-
-lemma sorted_perm_rel_exists (xs : inp list) :
+lemma total_ordering_to_perm_len_good (xs : inp list) :
   total_ordering xs =>
-  exists (perm : int list), sorted_perm_len_rel xs perm.
-proof. apply sorted_perm_exists. qed.
-
-lemma sorted_perm_len_rel_uniq (xs : inp list, perm1 perm2 : int list) :
-  total_ordering xs =>
-  sorted_perm_len_rel xs perm1 => sorted_perm_len_rel xs perm2 =>
-  perm1 = perm2.
+  total_ordering_to_perm_len xs \in perms_len.
 proof.
-move => tot_ord_xs [ispl1 srted1] [ispl2 srted2]. 
-rewrite (eq_sorted (cmp_of_rel xs) _ _ perm1 perm2) //.
-smt(cmp_total_ordering_trans tot_cmp_tot).
-smt(cmp_total_ordering_antisym tot_cmp_tot).
-smt(perm_eq_trans perm_eq_sym).
+move => tot_ord_xs.
+rewrite /total_ordering_to_perm_len /tsort /range_len /perms_len.
+rewrite allpermsP perm_eq_sym perm_sort.
 qed.
 
-(* now we can define our f and show it has the correct property *)
+lemma total_ordering_to_perm_len_injective (xs ys : inp list) :
+  total_ordering xs => total_ordering ys =>
+  total_ordering_to_perm_len xs = total_ordering_to_perm_len ys =>
+  xs = ys.
+proof.
+move => tot_ord_xs tot_ord_ys.
+rewrite /total_ordering_to_perm_len /range_len /tsort =>
+  eq_sort_xs_len_sort_ys_len.
+case (xs = ys) => [// | ne_xs_ys].
+have [i [ge0_i lt_i_size_xs]]
+     := diff_equal_size_index_diff xs ys _ _ => //.
+  rewrite total_ordering_size //.
+  rewrite total_ordering_size //.
+case (nth false xs i) => [xs_i_true | xs_i_false].
+(* nth false xs i *)
+pose j := (dec i).`1.
+pose k := (dec i).`2.
+have j_rng : 0 <= j < len.
+  rewrite /j dec_bounds_left.
+  smt(total_ordering_size).
+have k_rng : 0 <= k < len.
+  rewrite /k dec_bounds_right.
+  smt(total_ordering_size).
+have le_xs_j_k : rel xs j k.
+  rewrite /rel /j /k.
+  have -> : ((dec i).`1, (dec i).`2) = dec i by smt().
+  rewrite decK //.
+  smt(total_ordering_size).
+have lt_ys_k_j : ! rel ys j k.
+  rewrite /rel /j /k.
+  have -> : ((dec i).`1, (dec i).`2) = dec i by smt().
+  rewrite decK //.
+  smt(total_ordering_size).
+  smt().
+have sorted_sort_by_xs :
+      sorted (cmp_of_rel xs) (sort (cmp_of_rel xs) (range 0 len)).
+  rewrite sort_sorted.
+  move => x y; rewrite cmp_total_ordering_total tot_cmp_tot //.
+have sorted_sort_by_ys :
+      sorted (cmp_of_rel ys) (sort (cmp_of_rel ys) (range 0 len)).
+  rewrite sort_sorted.
+  move => x y; rewrite cmp_total_ordering_total tot_cmp_tot //.
+have := sorted_exists_nth (sort (cmp_of_rel xs) (range 0 len))
+        (cmp_of_rel xs) j k _ _ _ _ _ _ _ => //.
+  move => x y.
+  by rewrite cmp_total_ordering_total tot_cmp_tot.
+  move => y x z cmp_xs_x_y cmp_xs_y_z.
+  by rewrite (cmp_total_ordering_trans xs y) 1:tot_cmp_tot.
+  move => x y cmp_xs_x_y cmp_xs_y_z.
+  by rewrite (cmp_total_ordering_antisym xs x y) 1:tot_cmp_tot.
+  rewrite mem_sort; smt(mem_range).
+  rewrite mem_sort; smt(mem_range).
+move =>
+  [l m] [#] ge0_l lt_l_len ge0_m lt_m_len le_l_m
+  nth_sort_xs_l_eq_j nth_sort_xs_m_eq_k.
+have nth_sort_ys_l_eq_j :
+  nth witness (sort (cmp_of_rel ys) (range 0 len)) l = j.
+  by rewrite -eq_sort_xs_len_sort_ys_len nth_sort_xs_l_eq_j.
+have nth_sort_ys_m_eq_k :
+  nth witness (sort (cmp_of_rel ys) (range 0 len)) m = k.
+  by rewrite -eq_sort_xs_len_sort_ys_len nth_sort_xs_m_eq_k.
+have cmp_of_rel_ys_j_k : cmp_of_rel ys j k.
+  rewrite -nth_sort_ys_l_eq_j -nth_sort_ys_m_eq_k.
+  rewrite (sorted_nth _ (cmp_of_rel ys)) //.
+  move => x y.
+  by rewrite cmp_total_ordering_total tot_cmp_tot.
+  move => y x z cmp_ys_x_y cmp_ys_y_z.
+  by rewrite (cmp_total_ordering_trans ys y) 1:tot_cmp_tot.
+  move => x y cmp_ys_x_y cmp_ys_y_z.
+  by rewrite (cmp_total_ordering_antisym ys x y) 1:tot_cmp_tot.
+  smt().
+have // : rel ys j k by smt().
+(* ! nth false xs i *)
+have ys_i_true : nth false ys i by smt().
+pose j := (dec i).`1.
+pose k := (dec i).`2.
+have j_rng : 0 <= j < len.
+  rewrite /j dec_bounds_left.
+  smt(total_ordering_size).
+have k_rng : 0 <= k < len.
+  rewrite /k dec_bounds_right.
+  smt(total_ordering_size).
+have lt_xs_k_j : ! rel xs j k.
+  rewrite /rel /j /k.
+  have -> : ((dec i).`1, (dec i).`2) = dec i by smt().
+  rewrite decK //.
+  smt(total_ordering_size).
+have le_ys_j_k : rel ys j k.
+  rewrite /rel /j /k.
+  have -> : ((dec i).`1, (dec i).`2) = dec i by smt().
+  rewrite decK //.
+  smt(total_ordering_size).
+have sorted_sort_by_xs :
+      sorted (cmp_of_rel xs) (sort (cmp_of_rel xs) (range 0 len)).
+  rewrite sort_sorted.
+  move => x y.
+  rewrite cmp_total_ordering_total tot_cmp_tot //.
+have sorted_sort_by_ys :
+      sorted (cmp_of_rel ys) (sort (cmp_of_rel ys) (range 0 len)).
+  rewrite sort_sorted.
+  move => x y.
+  rewrite cmp_total_ordering_total tot_cmp_tot //.
+have := sorted_exists_nth (sort (cmp_of_rel ys) (range 0 len))
+        (cmp_of_rel ys) j k _ _ _ _ _ _ _ => //.
+  move => x y.
+  by rewrite cmp_total_ordering_total tot_cmp_tot.
+  move => y x z cmp_ys_x_y cmp_ys_y_z.
+  by rewrite (cmp_total_ordering_trans ys y) 1:tot_cmp_tot.
+  move => x y cmp_ys_x_y cmp_ys_y_z.
+  by rewrite (cmp_total_ordering_antisym ys x y) 1:tot_cmp_tot.
+  rewrite mem_sort; smt(mem_range).
+  rewrite mem_sort; smt(mem_range).
+move =>
+  [l m] [#] ge0_l lt_l_len ge0_m lt_m_len le_l_m
+  nth_sort_ys_l_eq_j nth_sort_ys_m_eq_k.
+have nth_sort_xs_l_eq_j :
+  nth witness (sort (cmp_of_rel xs) (range 0 len)) l = j.
+  by rewrite eq_sort_xs_len_sort_ys_len nth_sort_ys_l_eq_j.
+have nth_sort_xs_m_eq_k :
+  nth witness (sort (cmp_of_rel xs) (range 0 len)) m = k.
+  by rewrite eq_sort_xs_len_sort_ys_len nth_sort_ys_m_eq_k.
+have cmp_of_rel_xs_j_k : cmp_of_rel xs j k.
+  rewrite -nth_sort_xs_l_eq_j -nth_sort_xs_m_eq_k.
+  rewrite (sorted_nth _ (cmp_of_rel xs)) //.
+  move => x y.
+  by rewrite cmp_total_ordering_total tot_cmp_tot.
+  move => y x z cmp_xs_x_y cmp_xs_y_z.
+  by rewrite (cmp_total_ordering_trans xs y) 1:tot_cmp_tot.
+  move => x y cmp_xs_x_y cmp_xs_y_z.
+  by rewrite (cmp_total_ordering_antisym xs x y) 1:tot_cmp_tot.
+  smt().
+have // : rel xs j k by smt().
+qed.
+
+(* convert a permutation on 0 .. len - 1 to a total ordering *)
+
+op perm_len_to_total_ordering (ms : int list) : inp list =
+  mkseq
+  (fun (i : int) =>
+     index ((dec i).`1) ms <= index ((dec i).`2) ms)
+  arity.  
+
+lemma perm_len_to_total_ordering_good (ms : int list) :
+  ms \in perms_len =>
+  total_ordering (perm_len_to_total_ordering ms).
+proof.
+admit.
+qed.
+
+lemma perm_len_to_total_orderingK (ms : int list) :
+  total_ordering_to_perm_len (perm_len_to_total_ordering ms) = ms.
+proof.
+admit.
+qed.
+
+(* now we can define our f and show it has the correct property: *)
 
 type out = int list.
 
 op f (aux : aux, xs : inp list) : out option =
   if total_ordering xs
-  then Some (tsort xs (range 0 len) )
+  then Some (total_ordering_to_perm_len xs)
   else None.
 
 lemma f_prop (xs : inp list) :
   total_ordering xs =>
-  is_some (f () xs) /\ perm_eq (range 0 len) (oget (f () xs)) /\
+  is_some (f () xs) /\ perm_eq range_len (oget (f () xs)) /\
   tsorted xs (oget (f () xs)).
 proof.
 move => tot_ord_xs.
-split => [ /# | //  ].
+split => [/# |].
 split.
-rewrite /f /sorted_perm_len_rel tot_ord_xs => /=.
-smt(perm_eq_sym perm_sort).
-rewrite /tsort /f tot_ord_xs /tsorted /tsort => /=. 
-smt(sort_sorted cmp_total_ordering_total tot_cmp_tot).
+rewrite /f tot_ord_xs /=.
+rewrite perm_eq_sym /tsort perm_sort.
+rewrite /tsorted /f tot_ord_xs /= sort_sorted.
+move => i j.
+by rewrite cmp_total_ordering_total tot_cmp_tot.
 qed.
 
 lemma f_is_some (xs : inp list) :
@@ -378,10 +564,9 @@ have not_tot_ord_xs : ! total_ordering xs.
   qed.
 (* end of realization *)
 
-(* The adversary *)
+(* the adversary *)
 
 module Adv : ADV = {
-
   var inpss : inp list list  (* current possible lists of inputs *)
   
   proc init() : unit = {
@@ -390,21 +575,22 @@ module Adv : ADV = {
   }
 
   proc ans_query(i: int) : inp = {
-    (* var fst, snd : int ; *) (* stores the dec indices *)
-    var inpss_t, inpss_f : inp list list; (* two possible inpss sizes when the adversary answers true or false *) 
-    var ret : inp; 
+    (* two possible inpss elements when the adversary answers true or false *) 
+    var inpss_t, inpss_f : inp list list; 
+    var ret : inp;  (* return value *)
   
     inpss_t <- (filter_nth inpss i true);
-    inpss_f <- (filter_nth inpss i false);      
+    inpss_f <- (filter_nth inpss i false);
 
-    if (size(inpss_t) <= size(inpss_f)){
-      inpss <- filter_nth inpss i false;  (*answering false remains more possible inpust*)
+    if (size inpss_t <= size inpss_f) {   (* answering false keeps as least as *)
+      inpss <- filter_nth inpss i false;  (* many inputs lists as answering true *)
       ret <- false;     
-      }
+    }
     else {
-       (* this also covers:  1. the algorithm asks the rel of (i, i);
-                             2. (i, j) is asked before and this time (j, i);
-                             3. (i, j) = true, (j, k) = true,  this time asks (i,k), etc *)
+       (* this also covers:
+            1. the algorithm asks the rel of (i, i);
+            2. (i, j) is asked before and this time (j, i);
+            3. (i, j) = true, (j, k) = true, this time asks (i,k), etc. *)
       inpss <- filter_nth inpss i true;  
       ret <- true ;  
     }
@@ -412,94 +598,57 @@ module Adv : ADV = {
   }
 }.
 
-
-
-op tot2perm (xs: inp list) : int list =
-  if(total_ordering xs) then sort (cmp_of_rel xs) (range 0 len) else (range 0 len).
-
-op perms (n : int) : int list list = allperms (range 0 n).
-
-
-lemma tot2perm_injective:
-    lists_fun_injective ( init_inpss () ) (perms len) tot2perm.
-proof.
-rewrite /lists_fun_injective /init_inpss /good /tot2perm => x x' x_in_tot x'_in_tot. 
-rewrite mem_filter in x_in_tot.
-rewrite mem_filter in x'_in_tot.
-elim x_in_tot.
-elim x'_in_tot.
-simplify.
-move => tot_x' x'_in_all tot_x x_in_all. 
-  have -> : (if total_ordering x then sort (cmp_of_rel x) (range 0 len)
-     else range 0 len) =  sort (cmp_of_rel x) (range 0 len) by smt().
-  have -> : (if total_ordering x' then sort (cmp_of_rel x') (range 0 len)
-  else range 0 len) =  sort (cmp_of_rel x') (range 0 len) by smt().
-  have H: uniq (all_lists univ arity)by smt(all_list_uniq univ_uniq ge0_arity).
-case (x = x') => [ /# | x_neq_x' sorted_eq].
-  have H1: forall (i, j),  0 <= i<j < len /\   cmp_of_rel x i  j =  cmp_of_rel x' i j. 
-  admit.
-  have H2: forall (y, y'),  total_ordering y =>y \in all_lists univ arity => total_ordering y' => y' \in all_lists univ arity =>
-           y <> y' => sort (cmp_of_rel y) (range 0 len) <> sort (cmp_of_rel y') (range 0 len)  .
-  admit.
-smt().      
-qed.
-
-lemma tot2perm_surjective:
-     lists_fun_surjective ( init_inpss () ) (perms len) tot2perm.
-proof.
-rewrite /lists_fun_surjective /init_inpss /good /tot2perm => y y_in_perms_len /=.
-(* elim. *)
-(*   rewrite /perms. progress. search allperms. have H1 : perm_eq (range 0 len) [] by smt(allpermsP). *)
-(*   apply perm_eq_size in H1.  *)
-(* smt(gt0_len range_geq  size_range). *)
-case (exists x,x \in all_lists univ arity /\ total_ordering x /\ sort (cmp_of_rel x) (range 0 len) = y ) => [ // | not_x_map_y  ].
-smt(mem_filter).  
-rewrite negb_exists /= in not_x_map_y.
-    have H: forall x, x \in filter total_ordering (all_lists univ arity) <=> total_ordering x /\ x \in (all_lists univ arity) by smt(mem_filter).  
-   have H1: forall x, x \in filter total_ordering (all_lists univ arity)/\ (if total_ordering x then sort (cmp_of_rel x) (range 0 len) else range 0 len) =
-  y  <=> total_ordering x /\ x \in (all_lists univ arity) /\  sort (cmp_of_rel x) (range 0 len) = y by smt(mem_filter).
-  admit.
- qed.
-   
-  
-
-lemma uniq_init_inpss (aux:aux):
-  uniq (init_inpss aux).
+lemma uniq_init_inpss :
+  uniq (init_inpss ()).
 proof.    
-have H : inpss_invar aux (init_inpss aux) by smt(inpss_invar_init).
-rewrite /inpss_invar in H.
-smt().     
+smt(inpss_invar_init inpss_invar_uniq).
 qed.
 
-lemma tot2perm_init_inpss_perm_n (aux: aux):
-  lists_fun (init_inpss aux) (perms len) tot2perm. 
+lemma total_ordering_to_perm_len_lists_fun :
+  lists_fun (init_inpss ()) perms_len total_ordering_to_perm_len.
 proof.   
-rewrite /lists_fun /init_inpss /good /perms /tot2perm => [x x_in_init ].
-  have H1 : (if total_ordering x then sort (cmp_of_rel x) (range 0 len) else range 0 len) = sort (cmp_of_rel x) (range 0 len) by smt(mem_filter).  
-smt(perm_sort perm_eq_sym allpermsP). 
+rewrite /lists_fun /init_inpss /good => xs /=.
+rewrite mem_filter => [[tot_ord_xs _]].
+by rewrite total_ordering_to_perm_len_good.
 qed.
 
-lemma init_inpss_same_size_perms_len  : 
-   size (init_inpss ()) =  size (perms len). 
+lemma total_ordering_to_perm_len_lists_fun_injective :
+  lists_fun_injective (init_inpss ()) perms_len total_ordering_to_perm_len.
 proof.
-rewrite (uniq_sets_eq_size_if_injective_surjective (init_inpss ()) (perms len)   tot2perm ) //.
+rewrite /lists_fun_injective /init_inpss /good => xs ys.
+rewrite 2!mem_filter => [/= [tot_xs _] [tot_ys _]].
+by apply total_ordering_to_perm_len_injective.
+qed.
+
+lemma total_ordering_to_perm_len_lists_fun_surjective :
+  lists_fun_surjective (init_inpss ()) perms_len total_ordering_to_perm_len.
+proof.
+rewrite /lists_fun_surjective /init_inpss /good => ms ms_in_perms_len /=.
+exists (perm_len_to_total_ordering ms).
+split.
+rewrite mem_filter.
+split.
+by rewrite perm_len_to_total_ordering_good.
+rewrite all_lists_arity_have 1:ge0_arity.
+smt(perm_len_to_total_ordering_good total_ordering_size).
+rewrite allP => x _; rewrite /univ /#.
+by rewrite perm_len_to_total_orderingK.
+qed.
+
+lemma init_inpss_fact_len  : 
+  size (init_inpss ()) = fact len.
+proof.
+rewrite (uniq_sets_eq_size_if_injective_surjective (init_inpss ()) perms_len
+         total_ordering_to_perm_len) //.
 smt(uniq_init_inpss).
 rewrite /perms; smt(uniq_allperms).
-smt(tot2perm_init_inpss_perm_n).
-smt(tot2perm_injective).
-smt(tot2perm_surjective).
+by rewrite total_ordering_to_perm_len_lists_fun.
+by rewrite total_ordering_to_perm_len_lists_fun_injective.
+by rewrite total_ordering_to_perm_len_lists_fun_surjective.
+by rewrite size_perms_len.
 qed.
 
-lemma init_inpss_fact_len :
-  size (init_inpss () ) = fact len.
-proof.    
-rewrite init_inpss_same_size_perms_len /perms size_allperms_uniq.
-smt(range_uniq).
-smt(size_range gt0_len).
-qed.  
-
-
-  (* adversary is lossless *)
+(* adversary is lossless *)
 
 lemma Adv_init_ll : islossless Adv.init.
 proof.
@@ -511,96 +660,159 @@ proof.
 proc; auto.
 qed.
 
-    (* here is our main theorem: *)
+lemma filter_nth_size_b_not_b (inpss : inp list list, i : int, b : bool) :
+  0 <= i < arity =>
+  size inpss = size (filter_nth inpss i b) + size(filter_nth inpss i (!b)).
+proof.
+move => [ge0_i lt_i_arity].
+rewrite /filter_nth.
+elim inpss => [// | x xs IH /#].
+qed.
 
-lemma filter_p_not_p'_size:
-    forall (l: 'a list) (p p' : 'a -> bool),
-    (forall x, x \in l => p x = ! p' x) =>  size (filter p l) + size ( filter (p') l) = size  l.    
+lemma ge1_fact (n : int) :
+  0 <= n => 1 <= fact n.
 proof.
-progress.
-move: l H.
-elim =>  [//= | //= ].
-progress.
-case (p x) => [ p_x_true | p_x_false].
-have ->//= : ! (p' x) by smt(). 
-rewrite -H.
-smt().     
-smt().
-have ->//= : (p' x) by smt().   
-rewrite -H.
-smt().     
-smt().
-qed.     
-    
-lemma ge1_fact: forall n, 0<=n => 1<=fact n.
+elim n.
+by rewrite fact0.
+smt(factS fact1).
+qed.
+
+lemma ge1_fact_len :
+  1 <= fact len.
 proof.
-  elim => [// |//]. 
-  smt(fact0).
-  smt(factS fact1).
-qed.    
-  
+rewrite ge1_fact ge0_len.
+qed.
+
+lemma mem_implies_size_ge1 (x : 'a, ys : 'a list) :
+  x \in ys => 1 <= size ys.
+proof.
+case ys => [| /=].
+smt(in_nil).
+smt(size_ge0).
+qed.
+
+lemma inpss_not_done_iff (inpss : inp list list) :
+  inpss_invar () inpss =>
+  ! (inpss_done () inpss) <=> 2 <= size inpss.
+proof.
+move => [uniq_inpss all_f_is_some].
+rewrite /inpss_done.
+split.
+rewrite negb_forall /= => [[bs_opt /=]].
+rewrite negb_forall /= => [[cs_opt /=]].
+rewrite (implybE (bs_opt \in map (f tt) inpss)) negb_or /=.
+rewrite (implybE (cs_opt \in map (f tt) inpss)) negb_or /=.
+rewrite 2!mapP =>
+  [[[xs [xs_in_inpss bs_opt_eq_f_xs]]]
+   [[ys [ys_in_inpss cs_opt_eq_f_ys]]]
+   ne_bs_opt_cs_opt].
+have ne_xs_ys : xs <> ys by smt().
+have := splitPr inpss xs _ => // [[s1 s2] inpss_eq].
+rewrite inpss_eq size_cat /= addrC -addrA.
+have /# : 1 <= size s2 + size s1.
+have [] : ys \in s1 \/ ys \in xs :: s2 by rewrite -mem_cat /#.
+smt(mem_implies_size_ge1 size_ge0).
+smt(mem_implies_size_ge1 size_ge0).
+move : uniq_inpss all_f_is_some.
+case inpss => [// | xs inpss' /=].
+case inpss' => [// | ys inpss'' /=].
+rewrite negb_or.
+move =>
+  [#] ne_xs_ys xs_not_in_zs ys_not_in_inpss'' uniq_inpss''
+  [#] is_some_f_xs is_some_f_ys all_is_some_f_inpss'' _.
+have [bs f_xs_eq_Some_bs] : exists bs, f tt xs = Some bs.
+  exists (oget (f tt xs)); rewrite -some_oget /#.
+have [cs f_ys_eq_Some_cs] : exists cs, f tt ys = Some cs.
+  exists (oget (f tt ys)); rewrite -some_oget /#.
+rewrite negb_forall /=; exists (Some bs).
+rewrite negb_forall /=; exists (Some cs).
+rewrite implybE /= negb_or /=.
+split.
+left => /#.
+rewrite implybE /= negb_or /=.
+split.
+right; left => /#.
+have tot_ord_xs : total_ordering xs by smt().
+have tot_ord_ys : total_ordering ys by smt().
+move : ne_xs_ys.
+apply contra => eq_bs_cs.
+rewrite (total_ordering_to_perm_len_injective xs ys) //#.
+qed.
+
+lemma inpss_done_iff (inpss : inp list list) :
+  inpss_invar () inpss => 1 <= size inpss =>
+  inpss_done () inpss <=> size inpss = 1.
+proof.
+smt(inpss_not_done_iff).
+qed.
+
+lemma divpow2up_next_size_ge2 (inpss : inp list list, stage i : int, b : bool) :
+  0 <= stage => 0 <= i < arity => 2 <= size inpss =>
+  size (filter_nth inpss i (!b)) <= size (filter_nth inpss i b) =>
+  divpow2up (fact len) stage <= size inpss =>
+  divpow2up (fact len) (stage + 1) <= size (filter_nth inpss i b).
+proof.
+move =>
+  ge0_stage [ge0_i lt_i_arity] ge2_size_inpss le_size_filter_nth_not_b_b
+  le_dp2u_stage_size_inpss.
+rewrite (divpow2up_next_new_ub (size inpss)) 1:ge1_fact_len //.
+smt(filter_nth_size_b_not_b).
+qed.
+
+(* here is our main lemma: *)
+
 lemma G_Adv_main (Alg <: ALG{Adv}) : 
   hoare [G(Alg, Adv).main : true ==> res.`1 \/ int_log_up 2 (fact len) <= res.`2].
 proof.
-  proc.
+proc.
 seq 7 :
-  (inpss = init_inpss aux /\ error = false /\ don = inpss_done aux inpss /\
+  (inpss = init_inpss aux /\ !error /\ don = inpss_done aux inpss /\
    stage = 0 /\ queries = fset0 /\ Adv.inpss = init_inpss aux /\ aux = ()).
 wp.
 call (_ : true).
 inline Adv.init; auto. 
 while
-  (stage = card queries /\ queries_in_range queries /\
-   don = inpss_done aux inpss /\ divpow2up (fact len) stage <= size inpss /\ Adv.inpss = inpss).
-seq 1:
-  (stage = card queries /\ queries_in_range queries /\
-   don = inpss_done aux inpss /\ divpow2up (fact len) stage <= size inpss /\ Adv.inpss = inpss 
-   /\ !don /\ !error).
+  (stage = card queries /\ queries_in_range queries /\ Adv.inpss = inpss /\
+   inpss_invar () inpss /\  don = inpss_done aux inpss /\
+   divpow2up (fact len) stage <= size inpss).
+seq 1 :
+  (stage = card queries /\ queries_in_range queries /\ Adv.inpss = inpss /\
+   inpss_invar () inpss /\ don = inpss_done aux inpss /\
+   divpow2up (fact len) stage <= size inpss /\ !don /\ !error).
 call (_ : true); first auto.
 if.
 wp.
 call (_: true); first auto.
-sp. elim* => stage queries. 
+sp; elim* => stage' queries'.
 inline Adv.ans_query.
 sp 3.
 if.
 auto; progress [-delta]. 
 smt(fcardUindep1).
 smt(queries_in_range_add).
-rewrite /univ=> /=. 
-rewrite (divpow2up_next_new_ub (size inpss{hr})   (fact len) (card queries)  (size (filter_nth inpss{hr} i{hr} false)) ). 
-smt(ge1_fact ge1_len).
-smt(fcard_ge0).
-auto.
-  have filter_list_size :  size (filter_nth inpss{hr} i{hr} true) + size (filter_nth inpss{hr} i{hr} false) = size inpss{hr}.
-  rewrite /filter_nth => //=.
-  apply filter_p_not_p'_size.
-  smt().
-  smt().
+by rewrite inpss_invar_filter_nth.
+by rewrite divpow2up_next_size_ge2 1:fcard_ge0 // 1:-inpss_not_done_iff.
 auto; progress [-delta]. 
 smt(fcardUindep1).
 smt(queries_in_range_add).
-rewrite /univ=> /=. 
-rewrite (divpow2up_next_new_ub (size inpss{hr})   (fact len) (card queries)  (size (filter_nth inpss{hr} i{hr} true)) ). 
-smt(ge1_fact ge1_len).
-smt(fcard_ge0).
+by rewrite inpss_invar_filter_nth.
+rewrite divpow2up_next_size_ge2 1:fcard_ge0 // 1:-inpss_not_done_iff //#.
 auto.
-have filter_list_size :  size (filter_nth inpss{hr} i{hr} true) + size (filter_nth inpss{hr} i{hr} false) = size inpss{hr}.
-rewrite /filter_nth => //=. apply filter_p_not_p'_size.
-smt().
-smt().
-auto.
-auto; progress.
+auto; progress [-delta].
 smt(fcards0).
 smt(queries_in_range0).
-by rewrite divpow2up_start init_inpss_fact_len .
-rewrite negb_and in H.
-elim H => [ //= inpss_done | error ].
+rewrite inpss_invar_init.
+by rewrite divpow2up_start init_inpss_fact_len.
+rewrite negb_and /= in H0.
+elim H0 => [inpss_done | error].
 right.
 apply divpow2up_eq1_int_log_up_le.
 smt(ge1_fact ge1_len).
 smt(fcard_ge0).
-admit.  
+have ge1_dp2u : 1 <= divpow2up (fact len) (card queries0).
+  smt(divpow2up_ge1 ge1_fact_len fcard_ge0).
+apply ler_anti.
+rewrite ge1_dp2u /=.
+have /# : size inpss1 = 1 by rewrite -inpss_done_iff //#.
 by left. 
 qed.
-    
